linear quasi-injectivity

thys/Injectivity/LC.thy
@@ -37,7 +37,24 @@ lemma sameShape_map2: "sameShape xs (map f xs)"
 by (simp add: list_all2_conv_all_nth sameShape_def)
 
 hide_const linear
-definition "linear xs \<equiv> \<forall>ys. sameShape xs ys \<longrightarrow> (\<exists>f. map f xs = ys)"
+definition "linear (xs::('a :: var) list) \<equiv> \<forall>ys. sameShape xs ys \<longrightarrow> (\<exists>f. map f xs = ys)"
+
+lemma linear_imp: 
+assumes "linear xs" "sameShape xs ys" 
+shows "\<exists>f. map f xs = ys \<and> supp f \<subseteq> set xs"
+proof-
+  obtain f where ys: "map f xs = ys" using assms unfolding linear_def by auto
+  define g where "g \<equiv> \<lambda>x. if x \<in> set xs then f x else x"
+  show ?thesis
+  apply(rule exI[of _ g], safe)
+    subgoal unfolding ys[symmetric] apply(rule map_cong)
+      subgoal ..
+      subgoal unfolding g_def by auto .
+    subgoal unfolding g_def supp_def by (auto split: if_splits) .
+qed
+    
+  
+  
 
 (* generic for free BNFs: *)
 lemma cong_rev: "map f xs = map g xs \<Longrightarrow> x \<in> set xs \<Longrightarrow> f x = g x"
@@ -46,12 +63,24 @@ lemma cong_rev: "map f xs = map g xs \<Longrightarrow> x \<in> set xs \<Longrigh
 lemma cong_rev_id: "map f xs = xs \<Longrightarrow> x \<in> set xs \<Longrightarrow> f x = x"
   using cong_rev[of f xs id] by auto
 
-definition "match xs ys \<equiv> SOME f. map f xs = ys"
+definition "match (xs::('a :: var) list) ys \<equiv> SOME f. map f xs = ys \<and> (supp f \<subseteq> set xs)"
 
-lemma map_match:
-"linear xs \<Longrightarrow> sameShape xs ys \<Longrightarrow> map (match xs ys) xs = ys"  
-using someI[of "\<lambda>f. map f xs = ys"] unfolding linear_def match_def[symmetric] by auto
+lemma match:
+"linear xs \<Longrightarrow> sameShape xs ys \<Longrightarrow> map (match xs ys) xs = ys \<and> supp (match xs ys) \<subseteq> set xs"  
+using someI[of "\<lambda>f. map f xs = ys \<and> supp f \<subseteq> set xs"] 
+using linear_imp unfolding match_def by blast
 
+lemmas map_match = match[THEN conjunct1]
+lemmas supp_match = match[THEN conjunct2]
+
+lemma finite_supp_match:
+"linear xs \<Longrightarrow> sameShape xs ys \<Longrightarrow> finite (supp (match xs ys))"  
+by (metis List.finite_set match rev_finite_subset) 
+
+lemma card_supp_match:
+"linear (xs::('a :: var) list) \<Longrightarrow> sameShape xs ys \<Longrightarrow> 
+ |supp (match xs ys)| <o |UNIV::'a set|"  
+by (simp add: finite_supp_match infinite_UNIV)
 
 lemma match_unique:
 assumes "linear xs" "sameShape xs ys" "map f xs = ys" "x \<in> set xs"
@@ -131,7 +160,7 @@ using assms by (metis bij_not_equal_iff inj_onCI)
 
 
 (* *)
-definition swap :: "'a list \<Rightarrow> 'a list \<Rightarrow> ('a \<Rightarrow> 'a)" where
+definition swap :: "('a::var) list \<Rightarrow> 'a list \<Rightarrow> ('a \<Rightarrow> 'a)" where
 "swap xs ys x \<equiv> 
  if x \<in> set xs then match xs ys x 
  else if x \<in> set ys then match ys xs x 
@@ -140,11 +169,11 @@ definition swap :: "'a list \<Rightarrow> 'a list \<Rightarrow> ('a \<Rightarrow
 lemma supp_swap: "supp (swap xs ys) \<subseteq> set xs \<union> set ys"
   unfolding supp_def swap_def by auto
 
-lemma finite_supp_swap: "finite (supp (swap (xs::'a list) ys))"
+lemma finite_supp_swap: "finite (supp (swap xs ys))"
 by (meson List.finite_set finite_UnI finite_subset supp_swap)
 
-lemma card_supp_swap: "|supp (swap (xs::'a list) ys)| <o |UNIV::'a set|"
-sorry 
+lemma card_supp_swap: "|supp (swap (xs::('a::var) list) ys)| <o |UNIV::'a set|"
+by (simp add: finite_supp_swap infinite_UNIV)
 
 lemma imsupp_swap: "linear xs \<Longrightarrow> linear ys \<Longrightarrow> sameShape xs ys \<Longrightarrow> imsupp (swap xs ys) \<subseteq> set xs \<union> set ys"
 unfolding imsupp_def supp_def swap_def 
@@ -153,8 +182,12 @@ using match_set sameShape_sym by auto blast+
 lemma swap_sym: "set xs \<inter> set ys = {} \<Longrightarrow> swap xs ys = swap ys xs"
   unfolding supp_def swap_def fun_eq_iff by auto
 
-lemma swap_idem: "linear xs \<Longrightarrow> linear ys \<Longrightarrow> sameShape xs ys \<Longrightarrow> set xs \<inter> set ys = {} \<Longrightarrow> swap xs ys o swap xs ys = id"
-  sorry
+lemma swap_idem: 
+assumes "linear xs" "linear ys" "sameShape xs ys" "set xs \<inter> set ys = {}"
+shows "swap xs ys o swap xs ys = id"
+apply(rule ext)
+using assms unfolding swap_def 
+by simp (meson Int_emptyD match_rev match_set sameShape_sym)
 
 lemma bij_swap: "linear xs \<Longrightarrow> linear ys \<Longrightarrow> sameShape xs ys \<Longrightarrow> set xs \<inter> set ys = {} \<Longrightarrow> 
 bij (swap xs ys)"
@@ -188,6 +221,7 @@ lemma Lam_Inj_sym: "Lam (xs::'a::var list) t = Lam xs' t' \<longleftrightarrow>
      (\<forall>x\<in> FVars_term t' - set xs'. f' x = x) \<and> 
   permute_term f t = permute_term f' t')"
   sorry
+(* TODO: revive/adapt Jan's proof *)
 
 (* Getting rid of f and f' with the help of linearity (we can only do this 
 from the symmetric version! because we need disjointness in order to swap)*)
@@ -203,6 +237,7 @@ proof safe
   "linear ys" "sameShape ys xs" "sameShape ys xs'"
   "permute_term (swap xs ys) t = permute_term (swap xs' ys) t'"
   hence ss: "set ys \<inter> set xs = {}" "set ys \<inter> set xs' = {}" by auto
+  (* define sw where "sw \<equiv> \<lambda>z. if z \<in>" *)
   show "Lam xs t = Lam xs' t'"
   unfolding Lam_Inj_sym apply(rule exI[of _ ys]) 
   apply(rule exI[of _ "swap xs ys"]) apply(rule exI[of _ "swap xs' ys"])
@@ -212,12 +247,12 @@ proof safe
     subgoal using card_supp_swap .
     subgoal using supp_swap .
     subgoal using map_swap2 swap_sym by metis
-    subgoal using bij_swap swap_sym sorry (* need to work with a trimmed quasi-swap instead *)
+    subgoal by (metis Diff_iff IntE Int_emptyD Un_Int_eq(2,3) swap_def swap_sym ) 
     subgoal using bij_swap swap_sym by metis
     subgoal using card_supp_swap .
     subgoal using supp_swap by metis
     subgoal using map_swap2 swap_sym by metis
-    subgoal using bij_swap swap_sym sorry
+    subgoal by (metis Diff_iff Int_emptyD UnCI swap_def)
     subgoal by assumption .
 next
   assume "Lam xs t = Lam xs' t'" 
@@ -225,14 +260,28 @@ next
   ss: "set ys \<inter> (set xs \<union> set xs' \<union> FVars_term t \<union> FVars_term t') = {}" and 
   f: "bij f" "|supp f| <o |UNIV::'a set|" "supp f \<subseteq> set xs \<union> set ys" "map f xs = ys" 
     "\<forall>x\<in>FVars_term t - set xs. f x = x" and 
-  f': "bij f'" "|supp f'| <o |UNIV::'a set|" "supp f' \<subseteq> set xs' \<union> set ys \<and> map f' xs' = ys" and 
+  f': "bij f'" "|supp f'| <o |UNIV::'a set|" "supp f' \<subseteq> set xs' \<union> set ys \<and> map f' xs' = ys"  
     "\<forall>x\<in>FVars_term t' - set xs'. f' x = x" and
   p: "permute_term f t = permute_term f' t'" unfolding Lam_Inj_sym by blast
 
   have p1: "permute_term (swap xs ys) t = permute_term f t" 
-  apply(rule term.permute_cong) sorry
-  have p2: "permute_term (swap xs' ys) t' = permute_term f' t'" sorry
-
+  apply(rule term.permute_cong) 
+    subgoal by (metis Int_Un_emptyI1 bij_swap assms(1) bij_linear f(1,4) 
+       sameShape_map1 ss swap_sym)
+    subgoal using card_supp_swap .
+    subgoal by fact
+    subgoal by fact
+    subgoal by (metis (full_types) Diff_iff Int_Un_empty Int_Un_emptyI1 Int_commute 
+     Int_emptyD assms(1) bij_linear cong_rev f(1,4,5) map_swap1 sameShape_map2 ss swap_def) .
+  have p2: "permute_term (swap xs' ys) t' = permute_term f' t'"
+  apply(rule term.permute_cong) 
+    subgoal by (metis Int_Un_empty LC.bij_swap Un_commute assms(2) bij_linear f'(1,3) 
+      sameShape_map1 ss swap_sym)
+    subgoal using card_supp_swap .
+    subgoal by fact
+    subgoal by fact
+    subgoal by (metis (full_types) Diff_iff Int_Un_empty Int_Un_emptyI2 Int_commute 
+      Int_emptyD assms(2) bij_linear cong_rev f'(1,3,4) map_swap1 sameShape_map2 ss swap_def) .
   show "\<exists>ys. set ys \<inter> (set xs \<union> set xs' \<union> FVars_term t \<union> FVars_term t') = {} \<and> 
          linear ys \<and>
          sameShape ys xs \<and>
@@ -242,7 +291,33 @@ next
   apply (metis sameShape_map1) .
 qed
 
-(* Most user-friendly (lightest) version -- Does not make sense for lists, but works for linear types: *)
+(* And a version that works for renaming with matching: *)
+lemma Lam_Inj_sym_linear_vvsubst: 
+assumes "linear (xs::('a::var) list)" "linear xs'"
+shows "Lam xs t = Lam xs' t' \<longleftrightarrow> 
+(\<exists>ys.
+  set ys \<inter> (set xs \<union> set xs' \<union> FVars_term t \<union> FVars_term t') = {} \<and> 
+  linear ys \<and> sameShape ys xs \<and> sameShape ys xs' \<and>  
+  vvsubst (match xs ys) t = vvsubst (match xs' ys) t')"
+proof-
+  {fix t and xs::"'a::var list" and ys assume "set ys \<inter> (set xs \<union> FVars_term t) = {}"
+   "linear xs" "linear ys" "sameShape ys xs"
+   hence "vvsubst (match xs ys) t = permute_term (swap xs ys) t"
+   apply(subst term.vvsubst_permute[symmetric])
+     subgoal by (metis Int_Un_emptyI1 LC.bij_swap swap_sym)
+     subgoal using card_supp_swap .
+     subgoal apply(rule term.map_cong)
+       subgoal using card_supp_match sameShape_sym by blast
+       subgoal using card_supp_swap by blast
+       subgoal ..
+       subgoal by (metis (no_types, lifting) Int_Un_emptyI2 Int_emptyD in_mono match 
+         notin_supp sameShape_sym swap_def) . .
+  } note 1 = this
+  show ?thesis using assms 1[of _ xs t] 1 [of _ xs' t'] unfolding Lam_Inj_sym_linear[OF assms] 
+  apply(intro ex_cong1) by fastforce 
+qed
+
+(* Most user-friendly (lightest) versions -- do not make sense for lists, but works for linear types: *)
 corollary Lam_Inj_sym_linearType: 
 assumes linearType: "\<And>(xs::'a::var list). linear xs"
 shows "Lam (xs::'a::var list) t = Lam xs' t' \<longleftrightarrow> 
@@ -250,7 +325,16 @@ shows "Lam (xs::'a::var list) t = Lam xs' t' \<longleftrightarrow>
   set ys \<inter> (set xs \<union> set xs' \<union> FVars_term t \<union> FVars_term t') = {} \<and> 
   sameShape ys xs \<and> sameShape ys xs' \<and>  
   permute_term (swap xs ys) t = permute_term (swap xs' ys) t')"
-apply(subst Lam_Inj_sym_linear) using assms by auto
+  apply(subst Lam_Inj_sym_linear) using assms by auto
+
+corollary Lam_Inj_sym_linearType_vvsubst: 
+assumes linearType: "\<And>(xs::'a::var list). linear xs"
+shows "Lam (xs::'a::var list) t = Lam xs' t' \<longleftrightarrow> 
+(\<exists>ys.
+  set ys \<inter> (set xs \<union> set xs' \<union> FVars_term t \<union> FVars_term t') = {} \<and> 
+  sameShape ys xs \<and> sameShape ys xs' \<and>  
+  vvsubst (match xs ys) t = vvsubst (match xs' ys) t')"
+apply(subst Lam_Inj_sym_linear_vvsubst) using assms by auto
 
 (* The above instantiates nicely to:
 -- lambda-terms
